Add draft of lemmas with TODOs

TransVal/transval.v
@@ -1,11 +1,59 @@
-Require Import List.
-Require Import IL Exp Coherence sexp smt.
+Require Import List Specif.
+Require Import IL Annotation AutoIndTac Bisim Exp MoreExp Coherence Fresh sexp smt.
 
+Definition wrapEnv E :=
+fun (x:var) =>
+ match E x with
+|Some v => Some (natToBitvec v)
+|None => None
+end.
+
+(** TODO: Add constraint that s' must be an expression or a function call **)
 Lemma models_if_eval :
-forall s D E s' E', 
+forall s D E s' E' , 
 ssa  s D
--> ((nil, E,s) -> (nil, E',s'))
--> forall p, models E'  (translateStmt s p).
+-> star2 step (nil, E,s) nil (nil, E',s')
+-> forall p, models (wrapEnv E)  (translateStmt s p).
+
+Proof.
+admit.
+Qed.
+
+Definition smtCheck (s:stmt) (t:stmt) :=
+smtAnd (translateStmt s source) (translateStmt t target).
+
+(** TODO: Why doesn't this work? **)
+Fixpoint agreeOnList (E:senv) (XL:list var) (YL:list var):=
+True.
+(*
+match XL, YL with
+|nil , nil => True
+| nil, _ => False
+| _, nil => False
+| a::XL', b::YL' => match E a, E b with
+                        | Some v1, Some v2 => v1 = v2 /\ (agreeOnList E XL' YL')
+                        | None, None =>  (agreeOnList E XL' YL')
+                        | _,_ => False
+                    end
+end. *)
+
+(** TODO: Add constraint that XL and YL are the lists of the output variables of the corresponding programs **)
+Lemma not_smtCheck_entails_sat:
+forall s t E XL YL,
+~ (models E (smtCheck s t))
+-> (forall p V,  models V (translateStmt s p) -> models V (translateStmt s p))
+-> agreeOnList E XL YL.
+
+Proof.
+admit.
+Qed.
+
+(** TODO: make lemma definition work and add constraints **)
+Lemma unsat_is_semeq :
+forall s t s' t' E E1 E2 x y,
+(star2 step (nil, E , s) nil (nil, E1, s'))
+-> (star2 step (nil, E, t) nil (nil, E2, t'))
+-> E1 x = E2 y.
 (*
 *** Local Variables: ***
 *** coq-load-path: (("../" "Lvc")) ***
